LambdaP/Lemmas/Renaming.lean
@@ -57,20 +57,26 @@ theorem Sub.rename {Θ} {Γ : Ctx s1} {τ1 τ2 : Tau s1} (h : Sub Θ Γ τ1 τ2)
     simp only [Tau.rename, Ty.rename, Path.rename]
     rw [← Ty.open_rename_comm]
     exact Sub.sel_tm (h1.rename ρ)
-  | .sel_hi h1 h2 => fun ρ => by
+  | .sel_hi hr h1 h2 => fun ρ => by
     have h2' := h2.rename ρ
     simp only [Tau.rename] at h2'
     rw [← Ty.open_rename_comm, ← Ty.open_rename_comm] at h2'
     simp only [Tau.rename, Ty.rename]
     rw [← Ty.open_rename_comm]
-    exact Sub.sel_hi (h1.rename ρ) h2'
-  | .sel_lo hw h1 h2 => fun ρ => by
+    exact Sub.sel_hi (Path.root_isBound_rename hr) (h1.rename ρ) h2'
+  | .sel_lo hr hw h1 h2 => fun ρ => by
     have h2' := h2.rename ρ
     simp only [Tau.rename] at h2'
     rw [← Ty.open_rename_comm, ← Ty.open_rename_comm] at h2'
     simp only [Tau.rename, Ty.rename]
     rw [← Ty.open_rename_comm]
-    exact Sub.sel_lo (hw.rename ρ) (h1.rename ρ) h2'
+    exact Sub.sel_lo (Path.root_isBound_rename hr) (hw.rename ρ) (h1.rename ρ) h2'
+  | .sel_hi_loc hc hl => fun _ => by
+    simp only [Tau.rename, Ty.rename, Ty.fromClosed_rename]
+    exact Sub.sel_hi_loc hc.rename hl
+  | .sel_lo_loc hc hl => fun _ => by
+    simp only [Tau.rename, Ty.rename, Ty.fromClosed_rename]
+    exact Sub.sel_lo_loc hc.rename hl
   | .arrow h1 h2 => fun ρ => .arrow (h1.rename ρ) (h2.rename (Renaming.ext ρ))
   | .pair_tm h1 h2 => fun ρ => .pair_tm (h1.rename ρ) (h2.rename (Renaming.ext ρ))
   | .pair_ty h1 h2 => fun ρ => .pair_ty (h1.rename ρ) (h2.rename (Renaming.ext ρ))
